
Parte 1
$$
h^{2} +2h = h(h+2)
$$
$$
a^{2}+2ab+b^{2}
$$
$$
\frac{2ab}{2a}=b
$$
$$
b\to b^{2} = \left( \frac{2ab}{2a} \right)^{2}
$$
$$
\left( \frac{2h}{2\sqrt{ h^{2} }} \right)=1
$$
$$
1^{2}=1 = b
$$

$$
h^{2}+2h +1 - 1
$$
$$
(h^{2}+2h +1) - 1 = (h+1)^{2}-1 \to u = h+1
$$
$$
u^{2}-1 = (u+1)(u-1)
$$



$$
1p^{8}+64p^{4} \to \left( \frac{64p^{4}}{2\sqrt{ p^{8} }} \right)^{2} = 1024
$$
$$
p^{8}+64p^{4}+1024 - 1024 = (p^{8}+64p^{4}+1024) - 1024
$$
$$
(p^{4}+32)^{2}-1024 = (p^{4}+32-32)(p^{4}+32+32)=p^{4}(p^{4}+64)
$$



$$
144x^{5}+5x^{2} 
$$
$$
\frac{5x^{2}}{2\sqrt{ 144x^{5} }}=\frac{5x^{2}}{2\cdot 12 x^{ 5/2 }}=\frac{5}{24} x^{2-5/2} = \frac{5}{24}x^{-1/2} \to \left( \frac{5}{24}x^{-1/2} \right) ^{2}
$$
$$
\frac{25}{576}x^{-1} = \frac{25}{576} \frac{1}{x} 
$$
$$
144x^{5}+5x^{2}+\frac{25}{576} \frac{1}{x}  - \frac{25}{576} \frac{1}{x} \to \left( 144x^{5}+5x^{2}+\frac{25}{576} \frac{1}{x} \right)+\frac{25}{576}\frac{1}{x}
$$
$$
\left( 12x^{5/2}+\frac{5}{24} \frac{1}{x^{1/2}} \right) = \left( 12x^{5/2}+\frac{5}{24} \frac{1}{\sqrt{ x }} \right)^{2}-\frac{25}{576} \frac{1}{x} 
$$



Parte 2
$$
a^{2} + b^{2} \to a^{2}+2ab + b^{2}- 2ab = (a+b)^{2}-2ab
$$

$$
x^{2}+16 = x^{2} +2(\sqrt{ x })(\sqrt{ 16 })+16 - 2(\sqrt{ x })(\sqrt{ 16 })
$$
$$
x^{2}+8x+16 -8x = (x^{2}+8x+16)-16 = (x+4)^{2}-16
$$


$$
9u^{24} + 121v^{12} \to 9u^{24} + 2(\sqrt{ 9u^{24} })(\sqrt{ 121v^{12} }) + 121v^{12} - 2(\sqrt{ 9u^{24} })(\sqrt{ 121v^{12} })
$$
$$
9u^{24} +2(3u^{12})(11v^{6})+ 121v^{12} - 2(3u^{12})(11v^{6})
$$
$$
9u^{24} +66u^{12}v^{6}+ 121v^{12} - 66u^{12}v^{6}
$$
$$
(3u^{12}+11v^{6})-66u^{12}v^{6}
$$


$$
49w^{7}+\frac{48}{49}k^{2}
$$
$$
49w^{7}+ 2 (\sqrt{ 49w^{7} })\left( \sqrt{ \frac{48}{49}k^{2} } \right)+\frac{48}{49}k^{2} -  2 (\sqrt{ 49w^{7} })\left( \sqrt{ \frac{48}{49}k^{2} } \right)
$$

$$
49w^{7}+2\sqrt{ 49\cdot \frac{48}{49} k^{2} w^{7} } + \frac{48}{49}k^{2}   - 2\sqrt{ 49\cdot \frac{48}{49} k^{2} w^{7} } 
$$
$$
49w^{7}+8k\sqrt{ 3 w^{7}} + \frac{48}{49} k^{2} - 8k\sqrt{ 3 w^{7}}
$$

$$
\left( 49w^{7}+8k\sqrt{ 3 w^{7}} + \frac{48}{49} k^{2} \right) - 8k\sqrt{ 3 w^{7}}
$$
$$
\left( \sqrt{ 49w^{7} } + \sqrt{ \frac{48}{49}k^{2} } \right) ^{2} - 8k\sqrt{ 3 w^{7}}
$$

$$
\left( 7 w^{7/2}+\frac{4}{7}\sqrt{ 3 }k \right) ^{2} - 8\sqrt{ 3 }kw^{7/2}
$$
