$$
x^{2}+bx+c \to (x-h)(x-m)
$$
$$(x+2)(x-3)=x^{2}-x-6$$
$$
\begin{cases}
b=-1 \\
c=-6
\end{cases}
$$
$$
\begin{cases}
hm=c=-6 \\
h+m = b = -1
\end{cases}
$$
$$
\begin{cases}
(6)(-1) = -6 \\
6-1=5
\end{cases} \to \begin{cases}
(3)(-2)=-6 \\
3-2=1
\end{cases} \to \begin{cases}
(-3)(2)=-6 \\
-3+2=-1
\end{cases}
$$
$$
\begin{cases}
h=-3 \\
m=2
\end{cases}
$$
$$
(x+h)(x+m)=(x-3)(x+2)
$$


$$
j^{2}-32j+240 = (j+h)(j+m)
$$
$$
\begin{cases}
h+m=32 \\
hm= 240
\end{cases}
$$
$$
240=2^{4}\cdot 3 \cdot 5
$$
$$
\begin{cases}
16\cdot 15=240 \\
16+15=31
\end{cases} \to 
\begin{cases}
10\cdot 24=240 \\
10+24 = 34
\end{cases} \to
\begin{cases}
12\cdot 20=240 \\
12+20=32
\end{cases}
$$

$$
\begin{cases}
(-12)(-20)=240 \\
(-12)+(-20) = 32
\end{cases}
$$
$$
(j-20)(j-12)
$$



$$
p^{2}-53p-420 \to (p-h)(p+m)
$$
$$
\begin{cases}
(-h)(m)=-420 \\
(-h)+m = -53
\end{cases}
$$

$$
(p-60)(p-7)
$$

$$
\frac{t^{4}}{7}-\frac{6}{7} t^{3}-\frac{112}{7} t^{2} \to \frac{1}{7}t^{2}(t^{2}-6t-112) \to \frac{1}{7}t^{2}(t-h)(t+m)
$$

$$
\frac{1}{7}t^{2}(t-14)(t+8)
$$
