

$$
(a+b)^{2}=(a+b)(a+b)=a\cdot a + a\cdot b + b\cdot a + b\cdot b = a^{2} + 2ab + b^{2}
$$
$$
a^{2} + 2ab+b^{2} \to (a + b)^{2}
$$



EEE
$$
9x^{2}+12xy+4y^{2} \to \begin{cases}
a^{2}=9x^{2} \to a=\sqrt{ 9x^{2} }=3x \\
b^{2} = 4y^{2} \to b = \sqrt{ 4y^{2} } = 2y \\
2ab=2(3x)(2y)=12xy
\end{cases}
$$
$$
(a+b)^{2}=(3x+2y)^{2}
$$
$$
(3x+2y)^{2}=(3x+2y)(3x+2y)=3x\cdot 3x + 3x\cdot 2y + 2y \cdot 3x + 2y \cdot 2y
$$
$$
9x^{2}+12xy + 4y^{2}
$$


Facilisimo
$$
(j\sqrt{ 3 }-k\sqrt{ 5 })^{2} = (j\sqrt{ 3 }-k\sqrt{ 5 })(j\sqrt{ 3 }-k\sqrt{ 5 }) = 3j^{2}-2jk\sqrt{ 15 } + 5k^{2}
$$
$$
\begin{cases}
a^{2} = 3j^{2} \to a = \sqrt{ 3j^{2} } = j\sqrt{ 3 } \\
b^{2}= 5k^{2} \to b = \sqrt{ 5k^{2} } = k\sqrt{ 5 } \\
2ab = 2(j\sqrt{ 3 })(k\sqrt{ 5 })=2jk\sqrt{ 15 } \\
-2ab \to -(2jk\sqrt{ 15 })
\end{cases}
$$
$$
(j\sqrt{ 3 }-k\sqrt{ 5 })^{2}
$$
$$
(k\sqrt{ 5 }-j\sqrt{ 3 })^{2}
$$

$$
k\sqrt{ 5 } - j\sqrt{ 3 } = (k\sqrt{ 5 } - j\sqrt{ 3 }) \to -1(j\sqrt{ 3 }-k\sqrt{ 5 })
$$

$$
[(-1)(j\sqrt{ 3 }-k\sqrt{ 5 })]^{2} = (-1)^{2}(j\sqrt{ 3 }-k\sqrt{ 5 })^{2} = (j\sqrt{ 3 }-k\sqrt{ 5 })
$$


Facililismo verdad
$$
-25bm^{2}+4an^{2} + 25am^{2} -4bn^{2} -20amn + 20bmn
$$
$$
(-25bm^{2}-4bn^{2}+20bmn)+(4an^{2}+25am^{2}-20amn)
$$
$$
b(-25m^{2}-4n^{2}+20mn)+a(4n^{2}+25m^{2}-20mn)
$$

 $$
 -b(25m^{2}-20mn +4n^{2})+a(25m^{2}-20mn+4n^{2})
 $$
 $$
 (-b+a)(25m^{2}-20mn+4n^{2})
 $$
 $$
 (a-b)(5m-2n)^{2}
 $$
 


AGREGAR
$$
p^{4}+15p^{2}+36
$$
$$
k\to p^{2}
$$


$$
(p^{2})^{2}+15(p^{2})+36=0
$$
$$
k^{2}+15k+36=0
$$
$$(k+3)(k+12)$$
$$
(p^{2}+3)(p^{2}+12)
$$
