
$$
x{^2}-y{^2} = (x+y)(x-y)
$$
$$
y^{2}-x^{2} = (y+x)(y-x)
$$
$$
(x-y)(x+y)=x\cdot x + x\cdot y - y\cdot x + y\cdot y
$$
$$
x^{2}+xy-xy+y^{2} = x^{2}+y^{2}
$$


$$
x-y = (\sqrt{ x }-\sqrt{ y })(\sqrt{ x }+\sqrt{ y })
$$
$$
(\sqrt{ x }\sqrt{ x }+\sqrt{ x }\sqrt{ y } -\sqrt{ x }\sqrt{ y }-\sqrt{ y }\sqrt{ y })
$$
$$
x^{1/2}x^{1/2}- y^{1/2}y^{1/2}
$$
$$
x^{ \frac{1}{2}+\frac{1}{2} } - y^{ \frac{1}{2}+\frac{1}{2} }
$$
$$
x^{1}-y^{1} = x-y
$$

$$
81x^{8}-169 = ((81x^{8})^{1/2} \pm (196)^{1/2})
$$
$$
(9x^{4}+13)(9x^{4}-13)
$$



Combinados
$$
a^{2}+2ab+b^{2}-16
$$
$$
(a+b)^{2}-16 \to u = (a+b) \to u^{2}-16
$$
$$
(u+16)(u-16)
$$
$$
(a+b+16)(a+b-16)
$$


$$
343j^{9}+245j^{6}k-175j^{3}k^{2}-125k^{3}
$$
$$
j^{6}(343j^{3}+245k)-k^{2}(175j^{3}+125k)
$$
$$
7j^{6}(49j^{3}+35k)-5k^{2}(35j^{3}+25k)
$$
$$
7\cdot 7j^{6}(7j^{3}+5k)-5\cdot 5 k^{2}(7j^{3}+5k)
$$
$$
49j^{6}(7j^{3}+5k)-25k^{2}(7j^{3}+5k)
$$
$$
(7j^{3}+5k)(49j^{6}-25k^{2})
$$
$$
(7j^{3}+5k)(7j^{3}-5k)(7j^{3}+5k)
$$
$$
(7j^{3}+5k)^{2}(7j^{3}-5k)
$$
