$$
ax^{2}+bx+c =0
$$
$$
x=\frac{-b\pm \sqrt{ b^{2}-4ac }}{2a}
$$
$$
(x+h)(x+m)
$$

$$
\begin{cases}
a = 1 \\
b = -53 \\
c = -420
\end{cases}
$$


$$
\begin{cases}
\frac{-53+67}{2} \\
\frac{-53-67}{2} \end{cases}
$$

$$
\begin{cases}
\frac{14}{2} \\
\frac{-120}{2}\end{cases}
$$


$$
\begin{cases}
7 \\
-60\end{cases}
$$


$$
\mathbb{R}
\mathbb{C}
$$

$$
x=\frac{-(12)\pm \sqrt{ (12)^{2}-4(9)(5) }}{2(9)}
$$
$$
x=\frac{-12\pm \sqrt{ 144-180 }}{18}
$$
$$
x=\frac{-12\pm \sqrt{ -36 }}{18}
$$
$$
x=\frac{-12\pm \sqrt{ 36 }\sqrt{ -1 }}{18}
$$
$$
x=\frac{-12\pm 6i}{18}
$$

$$
x=-\frac{12}{18}\pm \frac{6i}{18}
$$
$$
x=-\frac{2}{3}\pm \frac{1}{3}
$$
$$
x=\frac{-2\pm 1i}{3} 
$$
$$
3x=-2\pm i
$$

$$
3x +2 \mp i = 0
$$

$$
(3x +2 - i)(3x +2 + i) = 0
$$



$$
375x^{2} -220x -91
$$


$$
\begin{cases}
a = 375 \\
b = -220 \\
c=91 \\

\end{cases}
$$

$$
x=-(-220)
$$


$$
\begin{cases}
\frac{220+430}{750} \\
\frac{220-430}{750}
\end{cases}
$$

$$

(25)(15)m=(25)(15)(\begin{cases}\frac{13}{15} \\ \frac{7}{25} \end{cases})
$$

$$
\left(m-\frac{13}{15}\right)\left(m+\frac{7}{25}\right)=0
$$

$$
(15)\left(m-\frac{13}{15}\rigth)(25)\left(m+\frac{7}{25}\right)=(15)(25)0
$$