$$
\begin{cases}
(a+b)^{3}=a^{3}+3a^{2}b+3ab^{2}+b^{3} \\
(a-b)^{3}=a^{3}-3a^{2}b+3ab^{2}-b^{3}
\end{cases}
$$



$$
(9u-2v)^{3}
$$


$$
\begin{cases}
a=9u \\
b=2v
\end{cases}
$$

$$
(9u)^{3}-3(9u)^{2}(2v)+3(9u)(2v)^{2}-(2v)^{2}
$$
$$
729u^{3}-18v(81u^{2})+29u(4v^{2})-8v^{3}
$$
$$
729u^{3}-1458u^{2}v+29uv^{2}-8v^{3}
$$



jdskflg
$$
5j^{9}+13k^{4}
$$
$$
\begin{cases}
a = 5j^{9} \\
b=13k^{4}
\end{cases}
$$

$$
(5j^{9})^{3}+3(5j^{9})^{2}(13k^{4})+3(5j^{9})(13k^{4})^{2}+(13k^{4})^{3}
$$
$$
125j^{27}+3(25j^{18})(13k^{4})+3(5j^{9})(169k^{8})+2197k^{12}
$$
$$
125j^{27}+975j^{18}k^{4}+2535j^{9}k^{8}+2197k^{12}
$$

jjfdkhgdfkl
$$
8u^{15}+108mp^{2}u^{10}+729m^{3}p^{6}+ 486m^{2}p^{4}u^{5}
$$

$$
8u^{15}+108mp^{2}u^{10}+ 486m^{2}p^{4}u^{5} +729m^{3}p^{6}
$$
$$
\begin{cases}
a^{3} = 8u^{15}  \\
b^{3} =729 m^{3}p^{6}
\end{cases}
$$
$$
\begin{cases}
\sqrt[3]{ a^{3} } = \sqrt[3]{ 8u^{15} }  \\
\sqrt[3]{ b^{3} } =\sqrt[3]{ 729 m^{3}p^{6} }
\end{cases}
$$

$$
\begin{cases}
a = 2u^{15/3} \\
b = 9 m^{3/3} p^{6/3}
\end{cases}
$$
$$
\begin{cases}
a = 2u^{5} \\
b = 9 mp^{2} 
\end{cases}
$$
$$
(a+b)^{3} = (2u^{5}+9mp^{2})^{3} \to ?
$$

$$
3a^{2}b = 3(2u^{5})^{2}(9mp^{2}) = 3(4u^{10})(9mp^{2})= 108mp^{2}u^{10}
$$
$$
3ab^{2} = 3(2u^{5})(9mp^{2})^{2} = 3(2u^{5})(81m^{2}p^{4})= 483m^{2}p^{4}u^{5}
$$
$$
(2u^{5}+9mp^{2})^{3}
$$
