$$
\begin{cases}
a^{3}+b^{3}=(a+b)(a^{2}-ab+b^{2}) \\
a^{3}-b^{3}=(a-b)(a^{2}+ab+b^{2})
\end{cases}
$$

$$
a^{3}\pm b^{3}=(a \pm b)(a^{2}\mp ab+b^{2})
$$


ejemplo 1
$$
125k^{3} + 8p^{9}
$$
$$
\begin{cases}
a^{3}=125k^{3} \\
b^{3} = 8p^{9} 
\end{cases}
$$


$$
\begin{cases}
\sqrt[3]{ a^{3} }=\sqrt[3]{ 125k^{3} } \\
\sqrt[3]{ b^{3} } = \sqrt[3]{ 8p^{9} } 
\end{cases}
$$

$$
\begin{cases}
a = 5k^{3/3} \\
b = 2p^{9/3}
\end{cases}
$$
$$
\begin{cases}
a = 5k \\
b = 2p^{3}

\end{cases}
$$
$$
(5k+2p^{3})[(5k)^{2}-(5k)(2p^{3})+(2p^{3})^{2}]
$$
$$
(5k+2p^{3})[25k^{2}-10kp^{3}+4p^{5}]
$$

ejemplo 2
$$
3p^{2}-u
$$
$$
\begin{cases}
a^{3}=3p^{2} \\
b^{3}=u
\end{cases}
$$

$$
\begin{cases}
\sqrt[3]{ a^{3} }=\sqrt[3]{ 3p^{2} } \\
\sqrt[3]{ b^{3} }=\sqrt[3]{ u }
\end{cases}
$$

$$
\begin{cases}
a=3^{1/3}p^{2/3} \\
b=u^{1/3}
\end{cases}
$$

$$
(3^{1/3}p^{2/3}-u^{1/3})[(\sqrt[3]{ 3 }p^{2/3})^{2}+(\sqrt[3]{ 3 }p^{2/3})(\sqrt[3]{ u })+(\sqrt[3]{ u })^{2}]
$$
$$
(3^{1/3}p^{2/3}-u^{1/3})
[3^{2/3}p^{4/3}+3^{1/3}p^{2/3}u^{1/3}+u^{2/3}]
$$
$$
(\sqrt[3]{ 3p^{2} }-\sqrt[3]{ u })[\sqrt[3]{ 3^{2} p^{4}}+\sqrt[3]{ 3p^{2} u} +\sqrt[3]{ u^{2} }]
$$
