
Ejemplo
$$
12ab+7bc+12a^{2}+19ac+7c^{2} \to (a+b+c)(12a+7c)
$$


$$
(j+k)(k-1)=jk-j+k^{2}-k=j(k-1)+k(k-1)
$$
$$
p=k-1 \to jp +kp =p(j+k)\to (k-1)(j+k)
$$
$$
j(k-1)+k(k-1) = (k-1)(j+k) 
$$

Ejemplo 1
$$
jk-k-j+k^{2} = jk-j+k^{2}-k=(jk-j)+(k^{2}-k)=j(k-1)+k(k-1)
$$
$$
u=k-1 \to ju +ku = u(j+k) = (k-1)(j+k)
$$
$$
j(k-1)+k(k-1)=(k-1)(j+k)
$$
Ejemplo 2

$$
l^{3}+l^{2}+l+1 = (l^{3}+l^{2})+(l+1)=l^{2}(l+1)+(l+1)=l^{2}(l+1)+1(l+1)
$$
$$
(l^{2}+1)(l+1)
$$



$$
(20m+30n{^2})(7p-9g)=140mp-180gm+210n^{2}p-270gn^{2}=140mp-270gn^{2}-180gm+210n^{2}p
$$
Ejemplo 3
$$
(140mp-180gm)+(210n^{2}p-270gn^{2})=m(140p-180g)+n^{2}(210p-270g)
$$
$$
10m(14p-18g)+10n^{2}(21p-27g)=2\cdot 10m(7p-9g)+10 \cdot 3 n^{2}(7p-9g)
$$
$$
20m(7p-9g)+30n^{2}(7p-9g) = (7p-9g)(20m+30n^{2})
$$

